theories/zoo_parabs/pool.v
@@ -1,9 +1,15 @@
 From zoo Require Import
   prelude.
 From zoo.common Require Import
-  countable.
+  countable
+  gmultiset
+  list.
 From zoo.iris.bi Require Import
   big_op.
+From zoo.iris.base_logic Require Import
+  lib.ghost_list
+  lib.mono_gmultiset
+  lib.saved_prop.
 From zoo.language Require Import
   notations.
 From zoo.diaframe Require Import
@@ -24,9 +30,9 @@ From zoo Require Import
   options.
 
 Implicit Types b : bool.
-Implicit Types l : location.
-Implicit Types v t ctx hub task fut waiter pred fn : val.
+Implicit Types v ctx hub task fut waiter pred fn : val.
 Implicit Types empty : emptiness.
+Implicit Types own : ownership.
 
 #[local] Definition max_round_noyield :=
   val_to_nat pool_max_round_noyield.
@@ -48,16 +54,55 @@ Qed.
 Opaque pool__code.pool_max_round_yield.
 Opaque max_round_yield.
 
+Record job := {
+  job_val : val ;
+  job_name : gname ;
+}.
+Implicit Types job local global : job.
+
+#[local] Instance job_inhabited : Inhabited job :=
+  populate {|
+    job_val := inhabitant ;
+    job_name := inhabitant ;
+  |}.
+#[local] Instance job_eq_dec : EqDecision job :=
+  ltac:(solve_decision).
+#[local] Instance job_countable :
+  Countable job.
+Proof.
+  solve_countable.
+Qed.
+
+Implicit Types jobs locals ulocals globals : gmultiset job.
+Implicit Types localss : list $ gmultiset job.
+
+Definition pool_scope :=
+  gmultiset job.
+
+#[global] Instance pool_scope_eq_dec : EqDecision pool_scope :=
+  _.
+#[global] Instance pool_scope_countable :
+  Countable pool_scope.
+Proof.
+  apply _.
+Qed.
+
 Class SchedulerG Σ `{zoo_G : !ZooG Σ} := {
+  #[local] pool_G_saved_prop_G :: SavedPropG Σ ;
   #[local] pool_G_domain_G :: DomainG Σ ;
   #[local] pool_G_ivar_G :: Ivar3G Σ ;
   #[local] pool_G_ws_hub_G :: WsHubStdG Σ ;
+  #[local] pool_G_jobs_G :: MonoGmultisetG Σ job ;
+  #[local] pool_G_locals_G :: GhostListG Σ (gmultiset job) ;
 }.
 
 Definition pool_Σ := #[
+  saved_prop_Σ ;
   domain_Σ ;
   ivar_3_Σ ;
-  ws_hub_std_Σ
+  ws_hub_std_Σ ;
+  mono_gmultiset_Σ job ;
+  ghost_list_Σ (gmultiset job)
 ].
 #[global] Instance subG_pool_Σ Σ `{zoo_G : !ZooG Σ} :
   subG pool_Σ Σ →
@@ -66,192 +111,1312 @@ Proof.
   solve_inG.
 Qed.
 
-Section pool_G.
-  Context `{pool_G : SchedulerG Σ}.
+Module base.
+  Section pool_G.
+    Context `{pool_G : SchedulerG Σ}.
 
-  Implicit Types Ψ Χ Ξ : val → iProp Σ.
+    Implicit Types t : location.
+    Implicit Types P Q : iProp Σ.
+    Implicit Types Ψ Χ Ξ : val → iProp Σ.
 
-  Record metadata := {
-    metadata_size : nat ;
-    metadata_hub : val ;
-    metadata_domains : val ;
-  }.
-  Implicit Types γ : metadata.
+    Record metadata := {
+      metadata_size : nat ;
+      metadata_hub : val ;
+      metadata_domains : val ;
+      metadata_jobs : gname ;
+      metadata_locals : gname ;
+    }.
+    Implicit Types γ : metadata.
+    Implicit Types γ_tokens : list gname.
 
-  #[local] Instance metadata_eq_dec : EqDecision metadata :=
-    ltac:(solve_decision).
-  #[local] Instance metadata_countable :
-    Countable metadata.
-  Proof.
-    solve_countable.
-  Qed.
+    #[global] Instance metadata_eq_dec : EqDecision metadata :=
+      ltac:(solve_decision).
+    #[global] Instance metadata_countable :
+      Countable metadata.
+    Proof.
+      solve_countable.
+    Qed.
 
-  Record context := {
-    context_size : nat ;
-    context_hub : val ;
-    context_id : nat ;
-  }.
-  Implicit Types 𝑐𝑡𝑥 : context.
+    #[local] Definition metadata_context γ (i : nat) :=
+      ( #γ.(metadata_size),
+        γ.(metadata_hub),
+        #i
+      )%V.
+    #[local] Instance metadata_context_inj γ :
+      Inj (=) (=) (metadata_context γ).
+    Proof.
+      rewrite /Inj. naive_solver.
+    Qed.
 
-  #[local] Coercion context_to_val 𝑐𝑡𝑥 :=
-    ( #𝑐𝑡𝑥.(context_size),
-      𝑐𝑡𝑥.(context_hub),
-      #𝑐𝑡𝑥.(context_id)
-    )%V.
+    #[local] Definition jobs_auth' γ_jobs own :=
+      mono_gmultiset_auth γ_jobs own.
+    #[local] Definition jobs_auth γ :=
+      jobs_auth' γ.(metadata_jobs).
+    #[local] Definition jobs_elem γ :=
+      mono_gmultiset_elem γ.(metadata_jobs).
 
-  #[local] Lemma context_to_val_inj' ctx 𝑐𝑡𝑥1 𝑐𝑡𝑥2 :
-    ctx = 𝑐𝑡𝑥1 →
-    ctx = 𝑐𝑡𝑥2 →
-    𝑐𝑡𝑥1 = 𝑐𝑡𝑥2.
-  Proof.
-    destruct 𝑐𝑡𝑥1, 𝑐𝑡𝑥2. naive_solver.
-  Qed.
-  #[local] Instance context_to_val_inj :
-    Inj (=) (=) context_to_val.
-  Proof.
-    intros ?*. eapply context_to_val_inj'; done.
-  Qed.
+    #[local] Definition jobs_finished jobs : iProp Σ :=
+      [∗ mset] job ∈ jobs,
+        ∃ P,
+        saved_prop job.(job_name) P ∗
+        □ P.
 
-  #[local] Definition context_consistent γ 𝑐𝑡𝑥 :=
-    γ.(metadata_size) = 𝑐𝑡𝑥.(context_size) ∧
-    γ.(metadata_hub) = 𝑐𝑡𝑥.(context_hub).
-  #[local] Instance : CustomIpatFormat "context_consistent" :=
-    "(
-      %H𝑐𝑡𝑥{}_size &
-      %H𝑐𝑡𝑥{}_hub
-    )".
+    #[local] Definition locals_auth' sz γ_locals ulocals : iProp Σ :=
+      ∃ localss,
+      ⌜length localss = S sz⌝ ∗
+      ghost_list_auth γ_locals localss ∗
+      ⌜ulocals = ⋃+ localss⌝.
+    #[local] Definition locals_auth γ :=
+      locals_auth' γ.(metadata_size) γ.(metadata_locals).
+    #[local] Instance : CustomIpatFormat "locals_auth" :=
+      "(
+        %localss{} &
+        %Hlocalss{} &
+        Hauth{_{}} &
+        ->
+      )".
+    #[local] Definition locals_at_running γ_locals i scope : iProp Σ :=
+      ∃ locals,
+      ghost_list_at γ_locals i Own (scope ⊎ locals) ∗
+      jobs_finished locals.
+    #[local] Instance : CustomIpatFormat "locals_at_running" :=
+      "(
+        %locals{} &
+        Hat{_{}} &
+        Hjobs_finished_locals{}
+      )".
+    #[local] Definition locals_at_finished γ_locals i : iProp Σ :=
+      ∃ locals,
+      ghost_list_at γ_locals i Own locals.
+    #[local] Instance : CustomIpatFormat "locals_at_finished" :=
+      "(
+        %locals{} &
+        Hat{_{}}
+      )".
+    #[local] Definition locals_at' γ_locals i scope : iProp Σ :=
+      match scope with
+      | Some scope =>
+          locals_at_running γ_locals i scope
+      | None =>
+          locals_at_finished γ_locals i
+      end.
+    #[local] Definition locals_at γ :=
+      locals_at' γ.(metadata_locals).
 
-  #[local] Definition task_model γ task Ψ : iProp Σ :=
-    ∀ 𝑐𝑡𝑥 empty,
-    ⌜context_consistent γ 𝑐𝑡𝑥⌝ -∗
-    ws_hub_std_owner γ.(metadata_hub) 𝑐𝑡𝑥.(context_id) Nonblocked empty -∗
-    WP task 𝑐𝑡𝑥 {{ v,
+    #[local] Definition globals_model_running γ globals : iProp Σ :=
+      ∃ jobs ulocals,
+      ⌜jobs = globals ⊎ ulocals⌝ ∗
+      jobs_auth γ Own jobs ∗
+      locals_auth γ ulocals.
+    #[local] Instance : CustomIpatFormat "globals_model_running" :=
+      "(
+        %jobs &
+        %ulocals &
+        -> &
+        Hjobs_auth &
+        Hlocals_auth
+      )".
+    #[local] Definition globals_model_finished γ : iProp Σ :=
+      [∗ list] i ∈ seq 0 (S γ.(metadata_size)),
+        locals_at γ i None.
+    #[local] Instance : CustomIpatFormat "globals_model_finished" :=
+      "Hlocals_ats".
+    #[local] Definition globals_model γ globals : iProp Σ :=
+        globals_model_running γ globals
+      ∨ globals_model_finished γ.
+    #[local] Instance : CustomIpatFormat "globals_model" :=
+      " [ (:globals_model_running {/>/})
+        | (:globals_model_finished)
+        ]
+      ".
+
+    #[local] Definition context_1 γ i (scope : pool_scope) : iProp Σ :=
       ∃ empty,
-      ws_hub_std_owner γ.(metadata_hub) 𝑐𝑡𝑥.(context_id) Nonblocked empty ∗
-      Ψ v
-    }}.
+      ws_hub_std_owner γ.(metadata_hub) i Nonblocked empty ∗
+      locals_at γ i (Some scope).
+    #[local] Instance : CustomIpatFormat "context_1" :=
+      "(
+        %empty{} &
+        Hhub_owner{_{}} &
+        Hlocals_at{_{}}
+      )".
 
-  #[local] Definition inv_inner γ : iProp Σ :=
-    ∃ tasks,
-    ws_hub_std_model γ.(metadata_hub) tasks ∗
-    [∗ mset] task ∈ tasks,
-      task_model γ task (λ _, True).
-  #[local] Instance : CustomIpatFormat "inv_inner" :=
-    "(
-      %tasks &
-      >Hhub_model &
-      Htasks
-    )".
-  #[local] Definition inv_1 γ : iProp Σ :=
-    inv (nroot.@"inv") (inv_inner γ).
-  #[local] Definition inv_2 γ : iProp Σ :=
-    ws_hub_std_inv γ.(metadata_hub) (nroot.@"hub") (S γ.(metadata_size)) ∗
-    inv_1 γ.
-  #[local] Instance : CustomIpatFormat "inv_2" :=
-    "(
-      #Hhub_inv{_{}} &
-      #Hinv{_{}}
-    )".
-  Definition pool_inv t sz : iProp Σ :=
-    ∃ l γ,
-    ⌜t = #l⌝ ∗
-    meta l nroot γ ∗
-    ⌜sz = γ.(metadata_size)⌝ ∗
-    inv_2 γ.
-  #[local] Instance : CustomIpatFormat "inv" :=
-    "(
-      %l{} &
-      %γ{} &
-      {%Heq{};->} &
-      #Hmeta{_{}} &
-      -> &
-      {#Hinv{};(:inv_2)}
-    )".
+    #[local] Definition task_model γ task Ψ : iProp Σ :=
+      ∀ i scope,
+      ⌜i ≤ γ.(metadata_size)⌝ -∗
+      context_1 γ i scope -∗
+      WP task (metadata_context γ i) {{ v,
+        context_1 γ i scope ∗
+        Ψ v
+      }}.
 
-  Definition pool_model t : iProp Σ :=
-    ∃ l γ empty doms,
-    ⌜t = #l⌝ ∗
-    meta l nroot γ ∗
-    l.[size] ↦□ #γ.(metadata_size) ∗
-    l.[hub] ↦□ γ.(metadata_hub) ∗
-    l.[domains] ↦□ γ.(metadata_domains) ∗
-    inv_2 γ ∗
-    ws_hub_std_owner γ.(metadata_hub) 0 Blocked empty ∗
-    array_model γ.(metadata_domains) DfracDiscarded doms ∗
-    [∗ list] dom ∈ doms,
-      domain_model dom itype_unit.
-  #[local] Instance : CustomIpatFormat "model" :=
-    "(
-      %l{} &
-      %γ{} &
-      %empty{} &
-      %doms{} &
-      {%Heq{};->} &
-      #Hmeta{_{}} &
-      #Hl{}_size &
-      #Hl{}_hub &
-      #Hl{}_domains &
-      {#Hinv{};(:inv_2)} &
-      Hhub{}_owner &
-      Hdomains{} &
-      Hdoms{}
-    )".
+    #[local] Definition inv_inner γ : iProp Σ :=
+      ∃ globals 𝑔𝑙𝑜𝑏𝑎𝑙𝑠,
+      ⌜𝑔𝑙𝑜𝑏𝑎𝑙𝑠 = gmultiset_map job_val globals⌝ ∗
+      globals_model γ globals ∗
+      ws_hub_std_model γ.(metadata_hub) 𝑔𝑙𝑜𝑏𝑎𝑙𝑠 ∗
+      [∗ mset] global ∈ globals,
+        task_model γ global.(job_val) (λ _,
+          ∃ P,
+          saved_prop global.(job_name) P ∗
+          ▷ □ P
+        ).
+    #[local] Instance : CustomIpatFormat "inv_inner" :=
+      "(
+        %globals &
+        %𝑔𝑙𝑜𝑏𝑎𝑙𝑠 &
+        >%H𝑔𝑙𝑜𝑏𝑎𝑙𝑠 &
+        >Hglobals_model &
+        >Hhub_model &
+        Hglobals
+      )".
+    #[local] Definition inv_1 γ : iProp Σ :=
+      inv (nroot.@"inv") (inv_inner γ).
+    #[local] Definition inv_2 γ : iProp Σ :=
+      ws_hub_std_inv γ.(metadata_hub) (nroot.@"hub") (S γ.(metadata_size)) ∗
+      inv_1 γ.
+    #[local] Instance : CustomIpatFormat "inv_2" :=
+      "(
+        #Hhub_inv{_{}} &
+        #Hinv{_{}}
+      )".
+    Definition pool_inv γ sz : iProp Σ :=
+      ⌜sz = γ.(metadata_size)⌝ ∗
+      inv_2 γ.
+    #[local] Instance : CustomIpatFormat "inv" :=
+      "(
+        -> &
+        {#Hinv_{};(:inv_2)}
+      )".
 
-  #[local] Definition context_1 γ 𝑐𝑡𝑥 : iProp Σ :=
-    ∃ empty,
-    ws_hub_std_owner 𝑐𝑡𝑥.(context_hub) 𝑐𝑡𝑥.(context_id) Nonblocked empty.
-  #[local] Instance : CustomIpatFormat "context_1" :=
-    "(
-      %empty{} &
-      Hhub_owner
-    )".
-  #[local] Definition context_2 γ 𝑐𝑡𝑥 : iProp Σ :=
-    ⌜context_consistent γ 𝑐𝑡𝑥⌝ ∗
-    inv_2 γ ∗
-    context_1 γ 𝑐𝑡𝑥.
-  #[local] Instance : CustomIpatFormat "context_2" :=
-    "(
-      (:context_consistent {//}) &
-      {#Hinv_{};(:inv_2)} &
-      { {lazy} H𝑐𝑡𝑥{}
-      ; {lazy} H𝑐𝑡𝑥
-      ; (:context_1 ={})
-      ; (:context_1)
-      }
-    )".
-  Definition pool_context t ctx : iProp Σ :=
-    ∃ l γ 𝑐𝑡𝑥,
-    ⌜t = #l⌝ ∗
-    meta l nroot γ ∗
-    ⌜ctx = 𝑐𝑡𝑥⌝ ∗
-    context_2 γ 𝑐𝑡𝑥.
-  #[local] Instance : CustomIpatFormat "context" :=
-    "(
-      %l{} &
-      %γ{} &
-      %𝑐𝑡𝑥{} &
-      {%Heq{};->} &
-      #Hmeta{_{}} &
-      {%H𝑐𝑡𝑥{}_eq;->} &
-      (:context_2 {//} {/lazy/})
-    )".
+    #[local] Definition context_finished γ i : iProp Σ :=
+      ws_hub_std_owner γ.(metadata_hub) i Nonblocked Empty ∗
+      locals_at γ i (Some ∅).
+    #[local] Instance : CustomIpatFormat "context_finished" :=
+      "(
+        Hhub_owner{_{}} &
+        Hlocals_at{_{}}
+      )".
+    #[local] Definition context_2 γ i scope : iProp Σ :=
+      ⌜i ≤ γ.(metadata_size)⌝ ∗
+      inv_2 γ ∗
+      context_1 γ i scope.
+    #[local] Instance : CustomIpatFormat "context_2" :=
+      "(
+        %Hi{} &
+        {#Hinv_{};(:inv_2)} &
+        { {lazy} Hctx{}
+        ; {lazy} Hctx
+        ; (:context_1 ={})
+        ; (:context_1)
+        }
+      )".
+    Definition pool_context γ ctx scope : iProp Σ :=
+      ∃ i,
+      ⌜ctx = metadata_context γ i⌝ ∗
+      context_2 γ i scope.
+    #[local] Instance : CustomIpatFormat "context" :=
+      "(
+        %i{} &
+        {%Heq{};->} &
+        (:context_2 {//} {/lazy/})
+      )".
 
-  Definition pool_future_inv t fut Ψ Ξ :=
-    ivar_3_inv fut Ψ Ξ (λ fut waiter,
-      ∀ ctx v,
-      pool_context t ctx -∗
+    #[local] Definition worker_post γ i res : iProp Σ :=
+      ⌜res = ()%V⌝ ∗
+      context_finished γ i.
+    #[local] Instance : CustomIpatFormat "worker_post" :=
+      "(
+        -> &
+        (:context_finished)
+      )".
+
+    Definition pool_model t γ : iProp Σ :=
+      ∃ empty doms,
+      ⌜length doms = γ.(metadata_size)⌝ ∗
+      t.[size] ↦□ #γ.(metadata_size) ∗
+      t.[hub] ↦□ γ.(metadata_hub) ∗
+      t.[domains] ↦□ γ.(metadata_domains) ∗
+      inv_2 γ ∗
+      array_model γ.(metadata_domains) DfracDiscarded doms ∗
+      ( [∗ list] i ↦ dom ∈ doms,
+        domain_model dom (worker_post γ (S i))
+      ) ∗
+      ws_hub_std_owner γ.(metadata_hub) 0 Blocked empty ∗
+      locals_at γ 0 (Some ∅).
+    #[local] Instance : CustomIpatFormat "model" :=
+      "(
+        %empty{} &
+        %doms{} &
+        %Hdoms{} &
+        #Hl{}_size &
+        #Hl{}_hub &
+        #Hl{}_domains &
+        {#Hinv{};(:inv_2)} &
+        Hdomains{} &
+        Hdoms{} &
+        Hhub{}_owner &
+        Hlocals_at{_{}}
+      )".
+
+    Definition pool_obligation γ P : iProp Σ :=
+      ∃ job,
+      jobs_elem γ job ∗
+      saved_prop job.(job_name) P.
+    #[local] Instance : CustomIpatFormat "obligation" :=
+      "(
+        %job{} &
+        Hjobs_elem{_job{}} &
+        Hjob{}
+      )".
+
+    Definition pool_finished γ : iProp Σ :=
+      ∃ jobs,
+      jobs_auth γ Discard jobs ∗
+      jobs_finished jobs.
+    #[local] Instance : CustomIpatFormat "finished" :=
+      "(
+        %jobs{} &
+        Hjobs_auth{_{}} &
+        Hjobs_finished{_jobs{}}
+      )".
+
+    #[local] Definition future_waiter γ fut waiter : iProp Σ :=
+      ∀ ctx scope v,
+      pool_context γ ctx scope -∗
       ivar_3_result fut v -∗
       WP waiter ctx v {{ res,
         ⌜res = ()%V⌝ ∗
-        pool_context t ctx
-      }}
-    )%I.
+        pool_context γ ctx scope
+      }}.
+    Definition pool_future_inv γ fut Ψ Ξ :=
+      ivar_3_inv fut Ψ Ξ (future_waiter γ).
+
+    Definition pool_future_consumer :=
+      ivar_3_consumer.
+
+    Definition pool_future_result :=
+      ivar_3_result.
+    Definition pool_future_finished fut : iProp Σ :=
+      ∃ v,
+      pool_future_result fut v.
+
+    #[global] Instance pool_future_proper γ fut :
+      Proper (
+        (pointwise_relation _ (≡)) ==>
+        (pointwise_relation _ (≡)) ==>
+        (≡)
+      ) (pool_future_inv γ fut).
+    Proof.
+      solve_proper.
+    Qed.
+
+    #[local] Instance globals_model_timeless γ globals :
+      Timeless (globals_model γ globals).
+    Proof.
+      apply _.
+    Qed.
+    #[global] Instance pool_future_result_timeless fut v :
+      Timeless (pool_future_result fut v).
+    Proof.
+      apply _.
+    Qed.
+
+    #[local] Instance jobs_elem_persistent γ job :
+      Persistent (jobs_elem γ job).
+    Proof.
+      apply _.
+    Qed.
+    #[local] Instance jobs_finished_persistent jobs :
+      Persistent (jobs_finished jobs).
+    Proof.
+      apply _.
+    Qed.
+    #[global] Instance pool_obligation_persistent γ P :
+      Persistent (pool_obligation γ P).
+    Proof.
+      apply _.
+    Qed.
+    #[global] Instance pool_finished_persistent γ :
+      Persistent (pool_finished γ).
+    Proof.
+      apply _.
+    Qed.
+    #[global] Instance pool_future_inv_persistent γ fut Ψ Ξ :
+      Persistent (pool_future_inv γ fut Ψ Ξ).
+    Proof.
+      apply _.
+    Qed.
+    #[global] Instance pool_future_result_persistent fut v :
+      Persistent (pool_future_result fut v).
+    Proof.
+      apply _.
+    Qed.
+
+    #[local] Lemma jobs_alloc :
+      ⊢ |==>
+        ∃ γ_jobs,
+        jobs_auth' γ_jobs Own ∅.
+    Proof.
+      apply mono_gmultiset_alloc.
+    Qed.
+    #[local] Lemma jobs_auth_discard γ jobs :
+      jobs_auth γ Own jobs ⊢ |==>
+      jobs_auth γ Discard jobs.
+    Proof.
+      apply mono_gmultiset_auth_persist.
+    Qed.
+    #[local] Lemma jobs_elem_valid γ own jobs job :
+      jobs_auth γ own jobs -∗
+      jobs_elem γ job -∗
+      ⌜job ∈ jobs⌝.
+    Proof.
+      apply mono_gmultiset_elem_valid.
+    Qed.
+    #[local] Lemma jobs_insert {γ jobs} 𝑗𝑜𝑏 P :
+      jobs_auth γ Own jobs ⊢ |==>
+        ∃ job,
+        ⌜job.(job_val) = 𝑗𝑜𝑏⌝ ∗
+        jobs_auth γ Own ({[+job+]} ⊎ jobs) ∗
+        jobs_elem γ job ∗
+        saved_prop job.(job_name) P.
+    Proof.
+      iIntros "Hauth".
+      iMod (saved_prop_alloc P) as "(%η & #Hη)".
+      pose job := {|
+        job_val := 𝑗𝑜𝑏 ;
+        job_name := η ;
+      |}.
+      iMod (mono_gmultiset_insert job with "Hauth") as "Hauth".
+      iDestruct (mono_gmultiset_elem_get job with "Hauth") as "#Helem"; first set_solver.
+      iFrameSteps.
+    Qed.
+    Opaque jobs_elem.
+
+    #[local] Lemma jobs_finished_empty :
+      ⊢ jobs_finished ∅.
+    Proof.
+      iApply (big_sepMS_empty with "[//]").
+    Qed.
+    #[local] Lemma jobs_finished_elem_of job jobs :
+      job ∈ jobs →
+      jobs_finished jobs ⊢
+        ∃ P,
+        saved_prop job.(job_name) P ∗
+        □ P.
+    Proof.
+      apply: big_sepMS_elem_of.
+    Qed.
+    #[local] Lemma jobs_finished_insert {jobs} job P :
+      jobs_finished jobs -∗
+      saved_prop job.(job_name) P -∗
+      □ P -∗
+      jobs_finished ({[+job+]} ⊎ jobs).
+    Proof.
+      iIntros "Hfinished #Hjob #HP".
+      iApply (big_sepMS_insert_2 with "Hfinished").
+      iSteps.
+    Qed.
+    #[local] Lemma jobs_finished_union localss :
+      ( [∗ list] locals ∈ localss,
+        jobs_finished locals
+      ) ⊢
+      jobs_finished (⋃+ localss).
+    Proof.
+      apply big_sepMS_disj_union_list_2.
+    Qed.
+    Opaque jobs_finished.
+
+    #[local] Lemma locals_alloc sz :
+      ⊢ |==>
+        ∃ γ_locals,
+        locals_auth' sz γ_locals ∅ ∗
+        [∗ list] i ∈ seq 0 (S sz),
+          locals_at' γ_locals i (Some ∅).
+    Proof.
+      iMod (ghost_list_alloc (replicate (S sz) ∅)) as "(%γ_locals & $ & Hats)".
+      iSplitR.
+      - iPureIntro. split.
+        + simpl_length.
+        + rewrite gmultiset_disj_union_list_replicate_empty //.
+      - iDestruct (big_sepL_replicate_1 with "Hats") as "Hats".
+        iApply (big_sepL_impl with "Hats"). iIntros "!> !> %i_ %i _ Hat".
+        iExists ∅. rewrite right_id. iFrame.
+        iApply jobs_finished_empty.
+    Qed.
+    #[local] Lemma locals_at_exclusive γ i scope1 scope2 :
+      locals_at γ i scope1 -∗
+      locals_at γ i scope2 -∗
+      False.
+    Proof.
+      all:
+        destruct scope1 as [scope1 |];
+        [ iIntros "(:locals_at_running =1)"
+        | iIntros "(:locals_at_finished =1)"
+        ].
+      all:
+        destruct scope2 as [scope2 |];
+        [ iIntros "(:locals_at_running =2)"
+        | iIntros "(:locals_at_finished =2)"
+        ].
+      all: iApply (ghost_list_at_exclusive with "Hat_1 Hat_2").
+    Qed.
+    #[local] Lemma locals_insert {γ ulocals i scope} local :
+      locals_auth γ ulocals -∗
+      locals_at γ i (Some scope) ==∗
+        locals_auth γ ({[+local+]} ⊎ ulocals) ∗
+        locals_at γ i (Some ({[+local+]} ⊎ scope)).
+    Proof.
+      iIntros "(:locals_auth) (:locals_at_running)".
+      iDestruct (ghost_list_lookup with "Hauth Hat") as %Hlookup.
+      iMod (ghost_list_update_at ({[+local+]} ⊎ scope ⊎ locals) with "Hauth Hat") as "($ & $)".
+      iFrameSteps; iPureIntro.
+      { simpl_length. }
+      { rewrite -assoc gmultiset_disj_union_list_insert_disj_union_l //. }
+    Qed.
+    #[local] Lemma locals_at_finish γ i local P scope :
+      locals_at γ i (Some ({[+local+]} ⊎ scope)) -∗
+      saved_prop local.(job_name) P -∗
+      □ P -∗
+      locals_at γ i (Some scope).
+    Proof.
+      iIntros "(:locals_at_running) Hlocal HP".
+      iDestruct (jobs_finished_insert with "Hjobs_finished_locals Hlocal HP") as "$".
+      rewrite (comm (⊎) {[+_+]} scope) assoc //.
+    Qed.
+    #[local] Lemma locals_kill γ ulocals :
+      locals_auth γ ulocals -∗
+      ( [∗ list] i ∈ seq 0 (S γ.(metadata_size)),
+        locals_at γ i (Some ∅)
+      ) -∗
+        locals_auth γ ulocals ∗
+        ( [∗ list] i ∈ seq 0 (S γ.(metadata_size)),
+          locals_at γ i None
+        ) ∗
+        jobs_finished ulocals.
+    Proof.
+      iIntros "(:locals_auth) Hats".
+      iDestruct (big_sepL_seq_exists with "Hats") as "(%localss_ & %Hlocalss_ & Hats)".
+      iDestruct (big_sepL_sep with "Hats") as "(Hats & Hjobs_finisheds)".
+      iEval (setoid_rewrite (left_id ∅ (⊎))) in "Hats".
+      iDestruct (ghost_list_auth_ats with "Hauth Hats") as %<-; first lia.
+      iSplitL "Hauth"; first iFrameSteps.
+      iDestruct (jobs_finished_union with "Hjobs_finisheds") as "$".
+      iDestruct (big_sepL_to_seq0 with "Hats") as "Hats".
+      iEval (rewrite Hlocalss) in "Hats".
+      iApply (big_sepL_impl with "Hats"). iIntros "!> %i_ %i _ (%locals & _ & $)".
+    Qed.
+    Opaque locals_auth'.
+    Opaque locals_at'.
+
+    #[local] Lemma globals_model_init γ :
+      jobs_auth γ Own ∅ -∗
+      locals_auth γ ∅ -∗
+      globals_model γ ∅.
+    Proof.
+      iIntros "Hjobs_auth Hlocals_auth".
+      iLeft. iExists ∅, ∅. iFrameSteps.
+    Qed.
+    #[local] Lemma globals_model_locals_at γ globals i scope :
+      i ≤ γ.(metadata_size) →
+      globals_model γ globals -∗
+      locals_at γ i scope -∗
+        globals_model_running γ globals ∗
+        locals_at γ i scope.
+    Proof.
+      iIntros "%Hi (:globals_model >) Hlocals_at".
+      - iFrameSteps.
+      - iDestruct (big_sepL_seq_lookup' i with "Hlocals_ats") as "Hlocals_at_"; first lia.
+        iDestruct (locals_at_exclusive with "Hlocals_at Hlocals_at_") as %[].
+    Qed.
+    #[local] Lemma globals_model_push {γ globals} 𝑔𝑙𝑜𝑏𝑎𝑙 P i scope :
+      i ≤ γ.(metadata_size) →
+      globals_model γ globals -∗
+      locals_at γ i scope ==∗
+        ∃ global,
+        ⌜global.(job_val) = 𝑔𝑙𝑜𝑏𝑎𝑙⌝ ∗
+        globals_model γ ({[+global+]} ⊎ globals) ∗
+        locals_at γ i scope ∗
+        jobs_elem γ global ∗
+        saved_prop global.(job_name) P.
+    Proof.
+      iIntros "%Hi Hglobals_model Hlocals_at".
+      iDestruct (globals_model_locals_at with "Hglobals_model Hlocals_at") as "((:globals_model_running) & $)"; first done.
+      iMod (jobs_insert 𝑔𝑙𝑜𝑏𝑎𝑙 P with "Hjobs_auth") as "(%global & % & Hjobs_auth & $ & $)".
+      iStep. iLeft. iFrameSteps. iPureIntro.
+      set_solver by lia.
+    Qed.
+    #[local] Lemma globals_model_pop {γ globals} global globals' i scope :
+      i ≤ γ.(metadata_size) →
+      globals = {[+global+]} ⊎ globals' →
+      globals_model γ globals -∗
+      locals_at γ i (Some scope) ==∗
+        globals_model γ globals' ∗
+        locals_at γ i (Some ({[+global+]} ⊎ scope)).
+    Proof.
+      iIntros (Hi ->) "Hglobals_model Hlocals_at".
+      iDestruct (globals_model_locals_at with "Hglobals_model Hlocals_at") as "((:globals_model_running) & Hlocals_at)"; first done.
+      iMod (locals_insert global with "Hlocals_auth Hlocals_at") as "(Hlocals_auth & $)".
+      iLeft. iFrameSteps. iPureIntro.
+      set_solver by lia.
+    Qed.
+    #[local] Lemma globals_model_kill γ :
+      globals_model γ ∅ -∗
+      ( [∗ list] i ∈ seq 0 (S γ.(metadata_size)),
+        locals_at γ i (Some ∅)
+      ) ==∗
+        ∃ jobs,
+        globals_model γ ∅ ∗
+        jobs_auth γ Discard jobs ∗
+        jobs_finished jobs.
+    Proof.
+      iIntros "Hglobals_model Hlocals_ats".
+
+      iAssert (
+        globals_model_running γ ∅ ∗
+        [∗ list] i ∈ seq 0 (S γ.(metadata_size)),
+          locals_at γ i (Some ∅)
+      )%I with "[-]" as "((:globals_model_running) & Hlocals_ats)".
+      { iDestruct (big_sepL_lookup_acc _ _ 0 with "Hlocals_ats") as "(Hlocals_at & Hlocals_ats)"; first done.
+        iDestruct (globals_model_locals_at with "Hglobals_model Hlocals_at") as "($ & Hlocals_at)"; first lia.
+        iApply ("Hlocals_ats" with "Hlocals_at").
+      }
+
+      rewrite (left_id ∅ (⊎)).
+
+      iDestruct (locals_kill with "Hlocals_auth Hlocals_ats") as "(_ & $ & $)".
+      iApply (jobs_auth_discard with "Hjobs_auth").
+    Qed.
+    Opaque globals_model.
+
+    Lemma pool_inv_agree γ sz1 sz2 :
+      pool_inv γ sz1 -∗
+      pool_inv γ sz2 -∗
+      ⌜sz1 = sz2⌝.
+    Proof.
+      iSteps.
+    Qed.
+
+    Lemma pool_obligation_finished γ P :
+      pool_obligation γ P -∗
+      pool_finished γ -∗
+      ▷ □ P.
+    Proof.
+      iIntros "(:obligation) (:finished)".
+      iDestruct (jobs_elem_valid with "Hjobs_auth Hjobs_elem") as %Helem.
+      iDestruct (jobs_finished_elem_of with "Hjobs_finished") as "(%P_ & Hjob_ & HP)"; first done.
+      iDestruct (saved_prop_agree with "Hjob Hjob_") as "Heq".
+      iModIntro. iRewrite "Heq" => //.
+    Qed.
+
+    Lemma pool_future_consumer_divide {γ fut Ψ Ξ Χ} Χs :
+      pool_future_inv γ fut Ψ Ξ -∗
+      pool_future_consumer fut Χ -∗
+      (∀ x, Χ x -∗ [∗ list] Χ ∈ Χs, Χ x) ={⊤}=∗
+      [∗ list] Χ ∈ Χs, pool_future_consumer fut Χ.
+    Proof.
+      apply ivar_3_consumer_divide.
+    Qed.
+    Lemma pool_future_consumer_split {γ fut Ψ Χ Ξ} Χ1 Χ2 :
+      pool_future_inv γ fut Ψ Ξ -∗
+      pool_future_consumer fut Χ -∗
+      (∀ v, Χ v -∗ Χ1 v ∗ Χ2 v) ={⊤}=∗
+        pool_future_consumer fut Χ1 ∗
+        pool_future_consumer fut Χ2.
+    Proof.
+      apply ivar_3_consumer_split.
+    Qed.
+
+    Lemma pool_future_result_agree fut v1 v2 :
+      pool_future_result fut v1 -∗
+      pool_future_result fut v2 -∗
+      ⌜v1 = v2⌝.
+    Proof.
+      apply ivar_3_result_agree.
+    Qed.
+
+    Lemma pool_future_inv_result γ fut Ψ Ξ v :
+      pool_future_inv γ fut Ψ Ξ -∗
+      pool_future_result fut v ={⊤}=∗
+      ▷ □ Ξ v.
+    Proof.
+      apply ivar_3_inv_result.
+    Qed.
+    Lemma pool_future_inv_result_consumer γ fut Ψ Ξ v Χ :
+      pool_future_inv γ fut Ψ Ξ -∗
+      pool_future_result fut v -∗
+      pool_future_consumer fut Χ ={⊤}=∗
+        ▷^2 Χ v ∗
+        ▷ □ Ξ v.
+    Proof.
+      apply ivar_3_inv_result_consumer.
+    Qed.
+
+    #[local] Lemma pool_context_spec {sz : Z} {hub} {i : Z} γ (i_ : nat) :
+      sz = γ.(metadata_size) →
+      hub = γ.(metadata_hub) →
+      i = i_ →
+      {{{
+        True
+      }}}
+        pool__code.pool_context #sz hub #i
+      {{{
+        RET metadata_context γ i_;
+        True
+      }}}.
+    Proof.
+      iSteps.
+    Qed.
+
+    #[local] Lemma pool_context_main_spec t γ :
+      {{{
+        t.[size] ↦□ #γ.(metadata_size) ∗
+        t.[hub] ↦□ γ.(metadata_hub)
+      }}}
+        pool_context_main #t
+      {{{
+        RET metadata_context γ 0;
+        True
+      }}}.
+    Proof.
+      iIntros "%Φ (Ht_size & Ht_hub) HΦ".
+
+      wp_rec. do 2 wp_load.
+      wp_apply (pool_context_spec with "[//] HΦ"); done.
+    Qed.
+
+    #[local] Lemma pool_execute_spec γ i scope task Ψ :
+      i ≤ γ.(metadata_size) →
+      {{{
+        context_1 γ i scope ∗
+        task_model γ task Ψ
+      }}}
+        pool_execute (metadata_context γ i) task
+      {{{ v,
+        RET v;
+        context_1 γ i scope ∗
+        Ψ v
+      }}}.
+    Proof.
+      iIntros "%Hi %Φ (Hctx & Htask) HΦ".
+
+      wp_rec.
+      wp_smart_apply (wp_wand with "(Htask [//] Hctx) HΦ").
+    Qed.
+
+    #[local] Lemma pool_worker_spec γ i :
+      {{{
+        context_2 γ i ∅
+      }}}
+        pool_worker (metadata_context γ i)
+      {{{ res,
+        RET res;
+        worker_post γ i res
+      }}}.
+    Proof.
+      iIntros "%Φ (:context_2 lazy=) HΦ".
+      iLöb as "HLöb".
+      iDestruct "Hctx" as "(:context_1)".
+
+      wp_rec. rewrite pool_max_round_noyield pool_max_round_yield.
+
+      awp_smart_apply (ws_hub_std_pop_steal_spec with "[$Hhub_inv $Hhub_owner]") without "HΦ"; [done | lia.. |].
+      iInv "Hinv" as "(:inv_inner)".
+      iAaccIntro with "Hhub_model"; first iSteps. iIntros ([𝑔𝑙𝑜𝑏𝑎𝑙 |]) "Hhub_model".
+
+      - iDestruct "Hhub_model" as "(%𝑔𝑙𝑜𝑏𝑎𝑙𝑠' & -> & Hhub_model)".
+        apply symmetry, gmultiset_map_disj_union_singleton_l_inv in H𝑔𝑙𝑜𝑏𝑎𝑙𝑠 as (global & globals' & -> & -> & ->).
+        iDestruct (big_sepMS_disj_union with "Hglobals") as "(Hglobal & Hglobals')".
+        iEval (rewrite big_sepMS_singleton) in "Hglobal".
+        iMod (globals_model_pop global with "Hglobals_model Hlocals_at") as "(Hglobals_model & Hlocals_at)"; [done.. |].
+        iSplitR "Hglobal Hlocals_at". { iFrameSteps. }
+        clear- Hi. iIntros "!> %empty (Hhub_owner & _) HΦ".
+
+        wp_smart_apply (pool_execute_spec with "[$]"); first done. clear- Hi. iIntros (res) "((:context_1) & (%P & Hglobal & HP))".
+        iDestruct (locals_at_finish with "Hlocals_at Hglobal HP") as "Hlocals_at".
+        wp_smart_apply ("HLöb" with "[$] HΦ").
+
+      - iSplitR "Hlocals_at". { iFrameSteps. }
+        clear- Hi. iIntros "!> %empty (Hhub_owner & ->) HΦ".
+
+        wp_smart_apply (ws_hub_std_block_spec with "[$Hhub_inv $Hhub_owner]"); first done.
+        iSteps.
+    Qed.
+
+    #[local] Lemma pool_drain_spec γ i :
+      {{{
+        context_2 γ i ∅
+      }}}
+        pool_drain (metadata_context γ i)
+      {{{ res,
+        RET res;
+        worker_post γ i res
+      }}}.
+    Proof.
+      iIntros "%Φ (:context_2 lazy=) HΦ".
+      iLöb as "HLöb".
+      iDestruct "Hctx" as "(:context_1)".
+
+      wp_rec.
+
+      awp_smart_apply (ws_hub_std_pop_spec with "[$Hhub_inv $Hhub_owner]") without "HΦ"; first done.
+      iInv "Hinv" as "(:inv_inner)".
+      iAaccIntro with "Hhub_model"; first iSteps. iIntros ([𝑔𝑙𝑜𝑏𝑎𝑙 |]) "Hhub_model".
+
+      - iDestruct "Hhub_model" as "(%𝑔𝑙𝑜𝑏𝑎𝑙𝑠' & -> & Hhub_model)".
+        apply symmetry, gmultiset_map_disj_union_singleton_l_inv in H𝑔𝑙𝑜𝑏𝑎𝑙𝑠 as (global & globals' & -> & -> & ->).
+        iDestruct (big_sepMS_disj_union with "Hglobals") as "(Hglobal & Hglobals')".
+        iEval (rewrite big_sepMS_singleton) in "Hglobal".
+        iMod (globals_model_pop global with "Hglobals_model Hlocals_at") as "(Hglobals_model & Hlocals_at)"; [done.. |].
+        iSplitR "Hglobal Hlocals_at". { iFrameSteps. }
+        clear- Hi. iIntros "!> Hhub_owner HΦ".
+
+        wp_smart_apply (pool_execute_spec with "[$]"); first done. clear- Hi. iIntros (res) "((:context_1) & (%P & Hglobal & HP))".
+        iDestruct (locals_at_finish with "Hlocals_at Hglobal HP") as "Hlocals_at".
+        wp_smart_apply ("HLöb" with "[$] HΦ").
+
+      - iSplitR "Hlocals_at". { iFrameSteps. }
+        clear- Hi. iIntros "!> Hhub_owner HΦ".
+
+        wp_smart_apply (ws_hub_std_block_spec with "[$Hhub_inv $Hhub_owner]"); first done.
+        iSteps.
+    Qed.
+
+    Lemma pool_create_spec sz :
+      (0 ≤ sz)%Z →
+      {{{
+        True
+      }}}
+        pool_create #sz
+      {{{ t γ,
+        RET #t;
+        pool_inv γ ₊sz ∗
+        pool_model t γ ∗
+        meta_token t ⊤
+      }}}.
+    Proof.
+      iIntros "%Hsz %Φ _ HΦ".
+
+      wp_rec.
+
+      wp_smart_apply (ws_hub_std_create_spec with "[//]") as (hub) "(#Hhub_inv & Hhub_model & Hhub_owners)"; first lia.
+      rewrite Z2Nat.inj_add // Nat.add_1_r.
+      iDestruct (big_sepL_seq_cons_1 with "Hhub_owners") as "(Hhub_owner & Hhub_owners)".
+
+      wp_smart_apply (ws_hub_std_block_spec with "[$Hhub_inv $Hhub_owner]") as "Hhub_owner"; first done.
+
+      iMod jobs_alloc as "(%γ_jobs & Hjobs_auth)".
+
+      iMod (locals_alloc ₊sz) as "(%γ_locals & Hlocals_auth & Hlocals_ats)".
+      iDestruct (big_sepL_seq_cons_1 with "Hlocals_ats") as "(Hlocals_at & Hlocals_ats)".
+
+      pose γ 𝑑𝑜𝑚𝑠 := {|
+        metadata_size := ₊sz ;
+        metadata_hub := hub ;
+        metadata_domains := 𝑑𝑜𝑚𝑠 ;
+        metadata_jobs := γ_jobs ;
+        metadata_locals := γ_locals ;
+      |}.
+
+      wp_smart_apply (array_unsafe_initi_spec_disentangled_strong'
+        ( λ 𝑑𝑜𝑚𝑠,
+          inv_1 (γ 𝑑𝑜𝑚𝑠)
+        )
+        ( λ 𝑑𝑜𝑚𝑠 i dom,
+          domain_model dom (worker_post (γ 𝑑𝑜𝑚𝑠) (S i))
+        )
+      with "[Hhub_model Hhub_owners Hjobs_auth Hlocals_auth Hlocals_ats]") as (𝑑𝑜𝑚𝑠 doms) "(%Hdoms & Hdomains & #Hinv & Hdoms)"; first done.
+      { iSplitR "Hhub_owners Hlocals_ats".
+
+        - iIntros "!> %𝑑𝑜𝑚𝑠".
+          iApply inv_alloc.
+          iDestruct (globals_model_init (γ 𝑑𝑜𝑚𝑠) with "Hjobs_auth Hlocals_auth") as "$".
+          iFrame. rewrite big_sepMS_empty //.
+
+        - iDestruct (big_sepL_sep_2 with "Hhub_owners Hlocals_ats") as "H".
+          iApply (big_sepL_impl_strong with "H").
+          { simpl_length. }
+          iIntros "!>" (k i1 i2 (-> & Hi1)%lookup_seq (-> & Hi2)%lookup_seq) "(Hhub_owner & Hlocals_at) %𝑑𝑜𝑚𝑠 #Hinv".
+
+          wp_smart_apply (domain_spawn_spec with "[Hhub_owner Hlocals_at]"); last iSteps. iIntros "%tid _".
+          iApply wp_thread_id_mono.
+
+          wp_smart_apply (pool_context_spec (γ 𝑑𝑜𝑚𝑠) (S k) with "[//]") as "_"; [naive_solver lia.. |].
+          wp_apply (pool_worker_spec with "[Hhub_owner Hlocals_at]"); first iFrameSteps.
+          iSteps.
+      }
+      iMod (array_model_persist with "Hdomains") as "#Hdomains".
+
+      wp_block t as "Hmeta" "(Ht_size & Ht_hub & Ht_domains & _)".
+      iMod (pointsto_persist with "Ht_size") as "#Ht_size".
+      iMod (pointsto_persist with "Ht_hub") as "#Ht_hub".
+      iMod (pointsto_persist with "Ht_domains") as "#Ht_domains".
+
+      iApply "HΦ".
+      iFrameSteps.
+    Qed.
+
+    Lemma pool_run_spec Ψ t γ task :
+      {{{
+        pool_model t γ ∗
+        ( ∀ ctx scope,
+          pool_context γ ctx scope -∗
+          WP task ctx {{ v,
+            pool_context γ ctx scope ∗
+            Ψ v
+          }}
+        )
+      }}}
+        pool_run #t task
+      {{{ v,
+        RET v;
+        pool_model t γ ∗
+        Ψ v
+      }}}.
+    Proof.
+      iIntros "%Φ ((:model) & Htask) HΦ".
+
+      wp_rec. wp_load.
+      wp_apply (ws_hub_std_unblock_spec with "[$Hhub_inv $Hhub_owner]") as "Hhub_owner"; first done.
+      wp_smart_apply (pool_context_main_spec with "[$]") as "_".
+
+      wp_smart_apply (pool_execute_spec _ _ _ _ Ψ with "[$Hhub_owner $Hlocals_at Htask]").
+      { lia. }
+      { iIntros "{%} %i %scope %Hi Hctx".
+        wp_apply (wp_wand with "(Htask [Hctx])") as (v) "((:context =1) & $)"; first iFrameSteps.
+        apply (inj _) in Heq1 as <-. iFrame.
+      }
+      clear- Hdoms. iIntros (v) "((:context_1) & HΨ)".
+
+      wp_load.
+      wp_apply (ws_hub_std_block_spec with "[$Hhub_inv $Hhub_owner]") as "Hhub_owner"; first done.
+      iSteps.
+    Qed.
+
+    Lemma pool_kill_spec t γ :
+      {{{
+        pool_model t γ
+      }}}
+        pool_kill #t
+      {{{
+        RET ();
+        pool_finished γ
+      }}}.
+    Proof.
+      iIntros "%Φ (:model) HΦ".
+
+      wp_rec. wp_load.
+      wp_apply (ws_hub_std_unblock_spec with "[$Hhub_inv $Hhub_owner]") as "Hhub_owner"; first done.
+      wp_smart_apply (pool_context_main_spec with "[$]") as "_".
+
+      wp_smart_apply (pool_drain_spec with "[$Hhub_owner $Hlocals_at]"); first iSteps.
+      clear- Hdoms. iIntros (res) "(:worker_post)".
+
+      wp_load.
+      wp_smart_apply (ws_hub_std_kill_spec with "Hhub_inv") as "_".
+      wp_load.
+
+      iApply wp_fupd.
+      wp_smart_apply (array_iter_spec_disentangled' (λ i _, context_finished γ (S i))%I with "[$Hdomains Hdoms]") as "(_ & Hdoms)".
+      { iApply (big_sepL_impl with "Hdoms"). iIntros "!> %i %dom _ Hdom".
+        wp_apply (domain_join_spec with "Hdom").
+        iSteps.
+      }
+
+      iDestruct (big_sepL_seq_index_2 γ.(metadata_size) with "Hdoms") as "Hdoms"; first lia.
+      iDestruct (big_sepL_seq_shift1_2 with "Hdoms") as "Hdoms".
+      iDestruct (big_sepL_seq_cons_2 with "Hdoms [$]") as "Hdoms".
+      iDestruct (big_sepL_sep with "Hdoms") as "(Hhub_owners & Hlocals_ats)".
+
+      iApply "HΦ".
+
+      iInv "Hinv" as "(:inv_inner)".
+      iDestruct (ws_hub_std_model_empty with "Hhub_inv Hhub_model [Hhub_owners]") as %->.
+      { iApply (big_sepL_impl with "Hhub_owners").
+        iSteps.
+      }
+      apply symmetry, gmultiset_map_empty_inv in H𝑔𝑙𝑜𝑏𝑎𝑙𝑠 as ->.
+      iMod (globals_model_kill _ with "Hglobals_model Hlocals_ats") as "(%jobs & Hglobals_model & #Hjobs_auth & #Hjobs_finished)".
+      iSplitL. { iFrameSteps. }
+      iSteps.
+    Qed.
+
+    Lemma pool_size_spec γ sz ctx scope :
+      {{{
+        pool_inv γ sz ∗
+        pool_context γ ctx scope
+      }}}
+        pool_size ctx
+      {{{
+        RET #sz;
+        pool_context γ ctx scope
+      }}}.
+    Proof.
+      iSteps.
+    Qed.
+
+    Lemma pool_async_silent_spec P γ ctx scope task :
+      {{{
+        pool_context γ ctx scope ∗
+        ( ∀ ctx scope,
+          pool_context γ ctx scope -∗
+          WP task ctx {{ res,
+            pool_context γ ctx scope ∗
+            ▷ □ P
+          }}
+        )
+      }}}
+        pool_async_silent ctx task
+      {{{
+        RET ();
+        pool_context γ ctx scope ∗
+        pool_obligation γ P
+      }}}.
+    Proof.
+      iIntros "%Φ ((:context) & Htask) HΦ".
+
+      wp_rec.
+
+      awp_smart_apply (ws_hub_std_push_spec with "[$Hhub_inv $Hhub_owner]") without "HΦ"; first done.
+      iInv "Hinv" as "(:inv_inner)".
+      iAaccIntro with "Hhub_model"; first iFrameSteps. iIntros "Hhub_model".
+      iMod (globals_model_push task P with "Hglobals_model Hlocals_at") as "(%global & %Hglobal & Hglobals_model & Hlocals_at & #Hjobs_elem & #Hglobal)"; first done.
+      iSplitR "Hlocals_at".
+      { iFrame. iSplitR "Htask".
+        - iPureIntro.
+          rewrite gmultiset_map_disj_union gmultiset_map_singleton.
+          congruence.
+        - iApply big_sepMS_singleton.
+          rewrite Hglobal. iSteps.
+      }
+      iSteps.
+    Qed.
+
+    Lemma pool_wait_until_spec P γ ctx scope pred :
+      {{{
+        pool_context γ ctx scope ∗
+        □ WP pred () {{ res,
+          ∃ b,
+          ⌜res = #b⌝ ∗
+          if b then P else True
+        }}
+      }}}
+        pool_wait_until ctx pred
+      {{{
+        RET ();
+        pool_context γ ctx scope ∗
+        P
+      }}}.
+    Proof.
+      iIntros "%Φ ((:context lazy=) & #Hpred) HΦ".
+      iLöb as "HLöb".
+      iDestruct "Hctx" as "(:context_1)".
+
+      wp_rec. rewrite pool_max_round_noyield.
+      wp_smart_apply (wp_wand with "Hpred") as (res) "(%b & -> & HP)".
+      destruct b; first iSteps.
+
+      awp_smart_apply (ws_hub_std_pop_steal_until_spec P with "[$Hhub_inv $Hhub_owner $Hpred]") without "HΦ"; [done.. |].
+      iInv "Hinv" as "(:inv_inner)".
+      iAaccIntro with "Hhub_model"; first iSteps. iIntros ([𝑔𝑙𝑜𝑏𝑎𝑙 |]) "Hhub_model".
+
+      - iDestruct "Hhub_model" as "(%𝑔𝑙𝑜𝑏𝑎𝑙𝑠' & -> & Hhub_model)".
+        apply symmetry, gmultiset_map_disj_union_singleton_l_inv in H𝑔𝑙𝑜𝑏𝑎𝑙𝑠 as (global & globals' & -> & -> & ->).
+        iDestruct (big_sepMS_disj_union with "Hglobals") as "(Hglobal & Hglobals')".
+        iEval (rewrite big_sepMS_singleton) in "Hglobal".
+        iMod (globals_model_pop global with "Hglobals_model Hlocals_at") as "(Hglobals_model & Hlocals_at)"; [done.. |].
+        iSplitR "Hglobal Hlocals_at". { iFrameSteps. }
+        clear- Hi. iIntros "!> %empty (Hhub_owner & _) HΦ".
+
+        wp_smart_apply (pool_execute_spec with "[$]"); first done. clear- Hi. iIntros (res) "((:context_1) & (%Q & Hglobal & HQ))".
+        iDestruct (locals_at_finish with "Hlocals_at Hglobal HQ") as "Hlocals_at".
+        wp_smart_apply ("HLöb" with "[$] HΦ").
+
+      - iSplitR "Hlocals_at". { iFrameSteps. }
+        iSteps.
+    Qed.
+
+    Lemma pool_wait_while_spec P γ ctx scope pred :
+      {{{
+        pool_context γ ctx scope ∗
+        □ WP pred () {{ res,
+          ∃ b,
+          ⌜res = #b⌝ ∗
+          if b then True else P
+        }}
+      }}}
+        pool_wait_while ctx pred
+      {{{
+        RET ();
+        pool_context γ ctx scope ∗
+        P
+      }}}.
+    Proof.
+      iIntros "%Φ (Hctx & #Hpred) HΦ".
+
+      wp_rec.
+      wp_smart_apply (pool_wait_until_spec with "[$Hctx] HΦ"). iModIntro.
+      wp_smart_apply (wp_wand with "Hpred") as (res) "(%b & -> & HP)".
+      destruct b; iSteps.
+    Qed.
+  End pool_G.
+
+  #[global] Opaque pool_scope.
+  #[global] Opaque pool_inv.
+  #[global] Opaque pool_model.
+  #[global] Opaque pool_context.
+  #[global] Opaque pool_obligation.
+  #[global] Opaque pool_finished.
+
+  Section pool_G.
+    Context `{pool_G : SchedulerG Σ}.
+
+    Implicit Types P Q : iProp Σ.
+    Implicit Types Ψ Χ Ξ : val → iProp Σ.
+
+    Lemma pool_async_spec Ψ Ξ γ ctx scope task :
+      {{{
+        pool_context γ ctx scope ∗
+        ( ∀ ctx scope,
+          pool_context γ ctx scope -∗
+          WP task ctx {{ v,
+            pool_context γ ctx scope ∗
+            ▷ Ψ v ∗
+            ▷ □ Ξ v
+          }}
+        )
+      }}}
+        pool_async ctx task
+      {{{ fut,
+        RET fut;
+        pool_context γ ctx scope ∗
+        pool_future_inv γ fut Ψ Ξ ∗
+        pool_future_consumer fut Ψ ∗
+        pool_obligation γ (pool_future_finished fut)
+      }}}.
+    Proof.
+      iIntros "%Φ (Hctx & Htask) HΦ".
+
+      wp_rec.
+      wp_smart_apply (ivar_3_create_spec Ψ Ξ with "[//]") as (ivar) "(#Hivar_inv & Hivar_producer & Hivar_consumer)".
+
+      wp_smart_apply (pool_async_silent_spec (
+        ivar_3_determined ivar
+      ) with "[$Hctx Htask Hivar_producer]") as "(Hctx & Hobligation)".
+      { clear ctx scope. iIntros "%ctx %scope Hctx".
+
+        wp_smart_apply (wp_wand with "(Htask Hctx)") as (v) "(Hctx & HΨ & HΞ)".
+        wp_smart_apply (ivar_3_set_spec with "[$Hivar_inv $Hivar_producer $HΨ $HΞ]") as (waiters) "(#Hivar_result & Hwaiters)".
+        wp_smart_apply (lst_iter_spec' (λ _ _, pool_context γ ctx scope)%I with "[$Hctx Hwaiters]") as "$"; try done.
+
+        iApply (big_sepL_impl with "Hwaiters").
+        iSteps.
+        rewrite /ivar_3_determined. iSteps.
+      }
+
+      iSteps.
+    Qed.
+
+    Lemma pool_wait_spec γ ctx scope fut Ψ Ξ :
+      {{{
+        pool_context γ ctx scope ∗
+        pool_future_inv γ fut Ψ Ξ
+      }}}
+        pool_wait ctx fut
+      {{{ v,
+        RET v;
+        £ 2 ∗
+        pool_context γ ctx scope ∗
+        pool_future_result fut v
+      }}}.
+    Proof.
+      iIntros "%Φ (Hctx & #Hivar_inv) HΦ".
+
+      wp_rec.
+
+      wp_smart_apply (pool_wait_until_spec (ivar_3_determined fut)%I with "[$Hctx]") as "(Hctx & %v & #Hivar_result)".
+      { iModIntro.
+        wp_smart_apply (ivar_3_is_set_spec with "Hivar_inv") as (b) "Hivar_result".
+        rewrite /ivar_3_determined. destruct b; iSteps.
+      }
+
+      wp_smart_apply (ivar_3_get_spec with "[$Hivar_inv $Hivar_result]") as "H£".
+      iSteps.
+    Qed.
+
+    Lemma pool_iter_spec γ ctx scope fut Ψ Ξ fn :
+      {{{
+        pool_context γ ctx scope ∗
+        pool_future_inv γ fut Ψ Ξ ∗
+        ( ∀ ctx scope v,
+          pool_context γ ctx scope -∗
+          pool_future_result fut v -∗
+          WP fn ctx v {{ res,
+            ⌜res = ()%V⌝ ∗
+            pool_context γ ctx scope
+          }}
+        )
+      }}}
+        pool_iter ctx fut fn
+      {{{
+        RET ();
+        pool_context γ ctx scope
+      }}}.
+    Proof.
+      iIntros "%Φ (Hctx & #Hivar_inv & Hfn) HΦ".
+
+      wp_rec.
+      wp_smart_apply (ivar_3_wait_spec with "[$Hivar_inv $Hfn]") as ([v |]) "H"; iSteps.
+    Qed.
+
+    Lemma pool_map_spec {γ ctx scope fut1 Ψ1 Ξ1} Ψ2 Ξ2 fn :
+      {{{
+        pool_context γ ctx scope ∗
+        pool_future_inv γ fut1 Ψ1 Ξ1 ∗
+        ( ∀ ctx scope v1,
+          pool_context γ ctx scope -∗
+          pool_future_result fut1 v1 -∗
+          WP fn ctx v1 {{ v2,
+            pool_context γ ctx scope ∗
+            ▷ Ψ2 v2 ∗
+            ▷ □ Ξ2 v2
+          }}
+        )
+      }}}
+        pool_map ctx fut1 fn
+      {{{ fut2,
+        RET fut2;
+        pool_context γ ctx scope ∗
+        pool_future_inv γ fut2 Ψ2 Ξ2 ∗
+        pool_future_consumer fut2 Ψ2
+      }}}.
+    Proof.
+      iIntros "%Φ (Hctx & #Hfut1_inv & Hfn) HΦ".
+
+      wp_rec.
+      wp_smart_apply (ivar_3_create_spec Ψ2 Ξ2 with "[//]") as (fut2) "(#Hivar2_inv & Hivar2_producer & Hivar2_consumer)".
+
+      wp_smart_apply (pool_iter_spec with "[$Hctx $Hfut1_inv Hfn Hivar2_producer]") as "Hctx".
+      { clear ctx scope. iIntros "%ctx %scope %v1 Hctx #Hfut1_result".
+
+        wp_smart_apply (wp_wand with "(Hfn Hctx Hfut1_result)") as (v2) "(Hctx & HΨ2 & HΞ2)".
+        wp_smart_apply (ivar_3_set_spec with "[$Hivar2_inv $Hivar2_producer $HΨ2 $HΞ2]") as (waiters) "(#Hivar2_result & Hwaiters)".
+        wp_smart_apply (lst_iter_spec' (λ _ _, pool_context γ ctx scope)%I with "[$Hctx Hwaiters]") as "$"; try done.
+
+        iApply (big_sepL_impl with "Hwaiters").
+        iSteps.
+      }
+
+      iSteps.
+    Qed.
+  End pool_G.
+
+  #[global] Opaque pool_future_inv.
+  #[global] Opaque pool_future_consumer.
+  #[global] Opaque pool_future_result.
+End base.
+
+From zoo_parabs Require
+  pool__opaque.
+
+Section pool_G.
+  Context `{pool_G : SchedulerG Σ}.
+
+  Implicit Types 𝑡 : location.
+  Implicit Types t : val.
+
+  Definition pool_inv t sz : iProp Σ :=
+    ∃ 𝑡 γ,
+    ⌜t = #𝑡⌝ ∗
+    meta 𝑡 nroot γ ∗
+    base.pool_inv γ sz.
+  #[local] Instance : CustomIpatFormat "inv" :=
+    "(
+      %𝑡{} &
+      %γ{} &
+      {%Heq{};->} &
+      #Hmeta{_{}} &
+      Hinv{_{}}
+    )".
+
+  Definition pool_context t ctx scope : iProp Σ :=
+    ∃ 𝑡 γ,
+    ⌜t = #𝑡⌝ ∗
+    meta 𝑡 nroot γ ∗
+    base.pool_context γ ctx scope.
+  #[local] Instance : CustomIpatFormat "context" :=
+    "(
+      %𝑡{} &
+      %γ{} &
+      {%Heq{};->} &
+      #Hmeta{_{}} &
+      Hctx{_{}}
+    )".
+
+  Definition pool_model t : iProp Σ :=
+    ∃ 𝑡 γ,
+    ⌜t = #𝑡⌝ ∗
+    meta 𝑡 nroot γ ∗
+    base.pool_model 𝑡 γ.
+  #[local] Instance : CustomIpatFormat "model" :=
+    "(
+      %𝑡{} &
+      %γ{} &
+      {%Heq{};->} &
+      #Hmeta{_{}} &
+      Hmodel{_{}}
+    )".
+
+  Definition pool_obligation t P : iProp Σ :=
+    ∃ 𝑡 γ,
+    ⌜t = #𝑡⌝ ∗
+    meta 𝑡 nroot γ ∗
+    base.pool_obligation γ P.
+  #[local] Instance : CustomIpatFormat "obligation" :=
+    "(
+      %𝑡{} &
+      %γ{} &
+      {%Heq{};->} &
+      #Hmeta{_{}} &
+      Hobligation{_{}}
+    )".
+
+  Definition pool_finished t : iProp Σ :=
+    ∃ 𝑡 γ,
+    ⌜t = #𝑡⌝ ∗
+    meta 𝑡 nroot γ ∗
+    base.pool_finished γ.
+  #[local] Instance : CustomIpatFormat "finished" :=
+    "(
+      %𝑡{} &
+      %γ{} &
+      {%Heq{};->} &
+      #Hmeta{_{}} &
+      Hfinished{_{}}
+    )".
+
+  Definition pool_future_inv t fut Ψ Ξ : iProp Σ :=
+    ∃ 𝑡 γ,
+    ⌜t = #𝑡⌝ ∗
+    meta 𝑡 nroot γ ∗
+    base.pool_future_inv γ fut Ψ Ξ.
+  #[local] Instance : CustomIpatFormat "future_inv" :=
+    "(
+      %𝑡{} &
+      %γ{} &
+      {%Heq{};->} &
+      #Hmeta{_{}} &
+      Hfut_inv{_{}}
+    )".
 
   Definition pool_future_consumer :=
-    ivar_3_consumer.
+    base.pool_future_consumer.
 
   Definition pool_future_result :=
-    ivar_3_result.
+    base.pool_future_result.
+  Definition pool_future_finished fut : iProp Σ :=
+    ∃ v,
+    pool_future_result fut v.
 
   #[global] Instance pool_future_proper t fut :
     Proper (
@@ -265,6 +1430,17 @@ Section pool_G.
 
   #[global] Instance pool_future_result_timeless fut v :
     Timeless (pool_future_result fut v).
+  Proof.
+    apply _.
+  Qed.
+
+  #[global] Instance pool_obligation_persistent t P :
+    Persistent (pool_obligation t P).
+  Proof.
+    apply _.
+  Qed.
+  #[global] Instance pool_finished_persistent t :
+    Persistent (pool_finished t).
   Proof.
     apply _.
   Qed.
@@ -285,7 +1461,18 @@ Section pool_G.
     ⌜sz1 = sz2⌝.
   Proof.
     iIntros "(:inv =1) (:inv =2)". simplify.
-    iDestruct (meta_agree with "Hmeta_1 Hmeta_2") as %<-. done.
+    iDestruct (meta_agree with "Hmeta_1 Hmeta_2") as %->.
+    iApply (base.pool_inv_agree with "Hinv_1 Hinv_2").
+  Qed.
+
+  Lemma pool_obligation_finished t P :
+    pool_obligation t P -∗
+    pool_finished t -∗
+    ▷ □ P.
+  Proof.
+    iIntros "(:obligation =1) (:finished =2)". simplify.
+    iDestruct (meta_agree with "Hmeta_1 Hmeta_2") as %->.
+    iApply (base.pool_obligation_finished with "Hobligation_1 Hfinished_2").
   Qed.
 
   Lemma pool_future_consumer_divide {t fut Ψ Ξ Χ} Χs :
@@ -294,7 +1481,8 @@ Section pool_G.
     (∀ x, Χ x -∗ [∗ list] Χ ∈ Χs, Χ x) ={⊤}=∗
     [∗ list] Χ ∈ Χs, pool_future_consumer fut Χ.
   Proof.
-    apply ivar_3_consumer_divide.
+    iIntros "(:future_inv) Hfut_consumer H".
+    iApply (base.pool_future_consumer_divide with "Hfut_inv Hfut_consumer H").
   Qed.
   Lemma pool_future_consumer_split {t fut Ψ Χ Ξ} Χ1 Χ2 :
     pool_future_inv t fut Ψ Ξ -∗
@@ -303,7 +1491,8 @@ Section pool_G.
       pool_future_consumer fut Χ1 ∗
       pool_future_consumer fut Χ2.
   Proof.
-    apply ivar_3_consumer_split.
+    iIntros "(:future_inv) Hfut_consumer H".
+    iApply (base.pool_future_consumer_split with "Hfut_inv Hfut_consumer H").
   Qed.
 
   Lemma pool_future_result_agree fut v1 v2 :
@@ -311,7 +1500,7 @@ Section pool_G.
     pool_future_result fut v2 -∗
     ⌜v1 = v2⌝.
   Proof.
-    apply ivar_3_result_agree.
+    apply base.pool_future_result_agree.
   Qed.
 
   Lemma pool_future_inv_result t fut Ψ Ξ v :
@@ -319,7 +1508,8 @@ Section pool_G.
     pool_future_result fut v ={⊤}=∗
     ▷ □ Ξ v.
   Proof.
-    apply ivar_3_inv_result.
+    iIntros "(:future_inv) Hfut_result".
+    iApply (base.pool_future_inv_result with "Hfut_inv Hfut_result").
   Qed.
   Lemma pool_future_inv_result' t fut Ψ Ξ v :
     £ 1 -∗
@@ -327,7 +1517,9 @@ Section pool_G.
     pool_future_result fut v ={⊤}=∗
     □ Ξ v.
   Proof.
-    apply ivar_3_inv_result'.
+    iIntros "H£ Hfut_inv Hfut_result".
+    iMod (pool_future_inv_result with "Hfut_inv Hfut_result") as "HΞ".
+    iApply (lc_fupd_elim_later with "H£ HΞ").
   Qed.
   Lemma pool_future_inv_result_consumer t fut Ψ Ξ v Χ :
     pool_future_inv t fut Ψ Ξ -∗
@@ -336,7 +1528,8 @@ Section pool_G.
       ▷^2 Χ v ∗
       ▷ □ Ξ v.
   Proof.
-    apply ivar_3_inv_result_consumer.
+    iIntros "(:future_inv) Hfut_result Hfut_consumer".
+    iApply (base.pool_future_inv_result_consumer with "Hfut_inv Hfut_result Hfut_consumer").
   Qed.
   Lemma pool_future_inv_result_consumer' t fut Ψ Ξ v Χ :
     £ 2 -∗
@@ -346,67 +1539,11 @@ Section pool_G.
       Χ v ∗
       □ Ξ v.
   Proof.
-    apply ivar_3_inv_result_consumer'.
-  Qed.
-
-  #[local] Lemma pool_execute_spec γ 𝑐𝑡𝑥 task Ψ :
-    {{{
-      context_2 γ 𝑐𝑡𝑥 ∗
-      task_model γ task Ψ
-    }}}
-      pool_execute 𝑐𝑡𝑥 task
-    {{{ v,
-      RET v;
-      context_1 γ 𝑐𝑡𝑥 ∗
-      Ψ v
-    }}}.
-  Proof.
-    iIntros "%Φ ((:context_2) & Htask) HΦ".
-
-    wp_rec.
-    wp_smart_apply (wp_wand with "(Htask [//] [Hhub_owner])").
-    { rewrite H𝑐𝑡𝑥_hub //. }
-    rewrite H𝑐𝑡𝑥_hub. iStepFrameSteps 3.
-  Qed.
-
-  #[local] Lemma pool_worker_spec {γ ctx} 𝑐𝑡𝑥 :
-    ctx = 𝑐𝑡𝑥 →
-    {{{
-      context_2 γ 𝑐𝑡𝑥
-    }}}
-      pool_worker ctx
-    {{{
-      RET ();
-      True
-    }}}.
-  Proof.
-    iIntros (->) "%Φ (:context_2 lazy=) HΦ".
-    iLöb as "HLöb".
-    iDestruct "H𝑐𝑡𝑥" as "(:context_1)".
-
-    wp_rec. rewrite pool_max_round_noyield pool_max_round_yield.
-    wp_pures. rewrite -H𝑐𝑡𝑥_hub.
-
-    awp_apply (ws_hub_std_pop_steal_spec with "[$Hhub_inv $Hhub_owner]") without "HΦ"; [done | lia.. |].
-    iInv "Hinv" as "(:inv_inner)".
-    iAaccIntro with "Hhub_model"; first iSteps. iIntros ([task |]) "Hhub_model !>".
-
-    - iDestruct "Hhub_model" as "(%tasks' & -> & Hhub_model)".
-      iDestruct (big_sepMS_disj_union with "Htasks") as "(Htask & Htasks)".
-      rewrite big_sepMS_singleton.
-      iSplitR "Htask"; first iSteps.
-      clear empty. iIntros "%empty (Hhub_owner & _) HΦ".
-
-      wp_smart_apply (pool_execute_spec with "[Hhub_owner $Htask]") as (res) "(H𝑐𝑡𝑥 & _)".
-      { iStep 2. rewrite H𝑐𝑡𝑥_hub. iFrame. }
-      wp_smart_apply ("HLöb" with "H𝑐𝑡𝑥 HΦ").
-
-    - iSplitL; first iSteps.
-      clear empty. iIntros "%empty (Hhub_owner & ->) HΦ".
-
-      wp_pures. rewrite -H𝑐𝑡𝑥_hub.
-      wp_apply (ws_hub_std_block_spec with "[$Hhub_inv $Hhub_owner]"); first done.
-      iSteps.
+    iIntros "(H£1 & H£2) Hfut_inv Hfut_result Hfut_consumer".
+    iMod (pool_future_inv_result_consumer with "Hfut_inv Hfut_result Hfut_consumer") as "H".
+    rewrite -bi.later_sep.
+    iMod (lc_fupd_elim_later with "H£1 H") as "(HΧ & $)".
+    iApply (lc_fupd_elim_later with "H£2 HΧ").
   Qed.
 
   Lemma pool_create_spec sz :
@@ -421,66 +1558,21 @@ Section pool_G.
       pool_model t
     }}}.
   Proof.
-    iIntros "%Hsz %Φ _ HΦ".
+    iIntros "% %Φ _ HΦ".
 
-    wp_rec. rewrite /pool__code.pool_context.
-
-    wp_smart_apply (ws_hub_std_create_spec with "[//]") as (hub) "(#Hhub_inv & Hhub_model & Hhub_owners)"; first lia.
-    rewrite Z2Nat.inj_add // Nat.add_1_r.
-    iDestruct (big_sepL_seq_cons_1 with "Hhub_owners") as "(Hhub_owner & Hhub_owners)".
-
-    wp_smart_apply (ws_hub_std_block_spec with "[$Hhub_inv $Hhub_owner]") as "Hhub_owner"; first done.
-
-    pose γ 𝑑𝑜𝑚𝑠 := {|
-      metadata_size := ₊sz ;
-      metadata_hub := hub ;
-      metadata_domains := 𝑑𝑜𝑚𝑠 ;
-    |}.
-
-    wp_smart_apply (array_unsafe_initi_spec_disentangled_strong'
-      (λ 𝑑𝑜𝑚𝑠, inv_1 (γ 𝑑𝑜𝑚𝑠))
-      (λ _ dom, domain_model dom itype_unit)
-    with "[Hhub_model Hhub_owners]") as (𝑑𝑜𝑚𝑠 doms) "(_ & Hdomains & #Hinv & Hdoms)"; first done.
-    { iSplitL "Hhub_model".
-
-      - iIntros "!> %𝑑𝑜𝑚𝑠".
-        iApply inv_alloc.
-        iFrame. rewrite big_sepMS_empty //.
-
-      - iApply (big_sepL_impl_strong with "Hhub_owners").
-        { simpl_length. }
-        iIntros "!>" (k i1 i2 (-> & Hi1)%lookup_seq (-> & Hi2)%lookup_seq) "Hhub_owner %𝑑𝑜𝑚𝑠 #Hinv".
-
-        wp_smart_apply (domain_spawn_spec itype_unit with "[Hhub_owner]"); last iSteps. iIntros "%tid _".
-        iApply wp_thread_id_mono.
-
-        pose 𝑐𝑡𝑥 := {|
-          context_size := ₊sz ;
-          context_hub := hub ;
-          context_id := S k ;
-        |}.
-        wp_smart_apply (pool_worker_spec 𝑐𝑡𝑥 with "[$Hinv $Hhub_owner]"); [| iSteps..].
-        { rewrite /context_to_val /=. repeat f_equal; lia. }
-    }
-    iMod (array_model_persist with "Hdomains") as "#Hdomains".
-
-    wp_block l as "Hmeta" "(Hl_size & Hl_hub & Hl_domains & _)".
-    iMod (pointsto_persist with "Hl_size") as "#Hl_size".
-    iMod (pointsto_persist with "Hl_hub") as "#Hl_hub".
-    iMod (pointsto_persist with "Hl_domains") as "#Hl_domains".
-
-    iMod (meta_set (γ 𝑑𝑜𝑚𝑠) with "Hmeta") as "#Hmeta"; first done.
-
+    iApply wp_fupd.
+    wp_apply (base.pool_create_spec with "[//]") as (𝑡 γ) "(Hinv & Hmodel & Hmeta)"; first done.
+    iMod (meta_set γ with "Hmeta") as "#Hmeta"; first done.
     iSteps.
   Qed.
 
   Lemma pool_run_spec Ψ t task :
     {{{
       pool_model t ∗
-      ( ∀ ctx,
-        pool_context t ctx -∗
+      ( ∀ ctx scope,
+        pool_context t ctx scope -∗
         WP task ctx {{ v,
-          pool_context t ctx ∗
+          pool_context t ctx scope ∗
           Ψ v
         }}
       )
@@ -494,28 +1586,13 @@ Section pool_G.
   Proof.
     iIntros "%Φ ((:model) & Htask) HΦ".
 
-    wp_rec. rewrite /pool__code.pool_context.
-    wp_load.
-    wp_apply (ws_hub_std_unblock_spec with "[$Hhub_inv $Hhub_owner]") as "Hhub_owner"; first done.
-    do 2 wp_load.
-
-    pose 𝑐𝑡𝑥 := {|
-      context_size := γ.(metadata_size) ;
-      context_hub := γ.(metadata_hub) ;
-      context_id := 0 ;
-    |}.
-    wp_smart_apply (pool_execute_spec _ 𝑐𝑡𝑥 _ Ψ with "[$Hhub_owner Htask]") as (v) "{%} ((:context_1 =1) & HΨ)".
-    { iSplit.
-      - iFrame "#" => //.
-      - iIntros "{%} %𝑐𝑡𝑥 %empty (:context_consistent) Hhub_owner".
-        wp_apply (wp_wand with "(Htask [Hhub_owner])") as (v) "((:context =1) & $)".
-        { iStep 5. rewrite H𝑐𝑡𝑥_hub. iFrame. }
-        apply (inj context_to_val) in H𝑐𝑡𝑥1_eq as <-.
-        rewrite H𝑐𝑡𝑥_hub. iSteps.
+    wp_apply (base.pool_run_spec Ψ with "[$Hmodel Htask]").
+    { iIntros "%ctx %scope Hctx".
+      wp_apply (wp_wand with "(Htask [$Hctx])") as (v) "((:context =1) & $)"; first iSteps.
+      simplify.
+      iDestruct (meta_agree with "Hmeta Hmeta_1") as %->. iClear "Hmeta".
+      iFrame.
     }
-
-    wp_load.
-    wp_apply (ws_hub_std_block_spec with "[$Hhub_inv $Hhub_owner]") as "Hhub_owner"; first done.
     iSteps.
   Qed.
 
@@ -526,118 +1603,66 @@ Section pool_G.
       pool_kill t
     {{{
       RET ();
-      True
+      pool_finished t
     }}}.
   Proof.
     iIntros "%Φ (:model) HΦ".
 
-    wp_rec. wp_load.
-    wp_smart_apply (ws_hub_std_kill_spec with "Hhub_inv") as "_".
-    wp_load.
-    wp_smart_apply (array_iter_spec_disentangled' (λ _ _, True)%I with "[$Hdomains Hdoms]"); last iSteps.
-    iApply (big_sepL_impl with "Hdoms"). iIntros "!> %i %dom _ Hdom".
-    wp_apply (domain_join_spec with "Hdom").
+    wp_apply (base.pool_kill_spec with "Hmodel").
     iSteps.
   Qed.
 
-  Lemma pool_size_spec t sz ctx :
+  Lemma pool_size_spec t sz ctx scope :
     {{{
       pool_inv t sz ∗
-      pool_context t ctx
+      pool_context t ctx scope
     }}}
       pool_size ctx
     {{{
       RET #sz;
-      True
+      pool_context t ctx scope
     }}}.
   Proof.
-    iIntros "%Φ ((:inv =1) & (:context =2)) HΦ". simplify.
-    iDestruct (meta_agree with "Hmeta_1 Hmeta_2") as %<-. iClear "Hmeta_2".
-    rewrite H𝑐𝑡𝑥2_size. iSteps.
+    iIntros "%Φ ((:model =1) & (:context =2)) HΦ". simplify.
+    iDestruct (meta_agree with "Hmeta_1 Hmeta_2") as %->. iClear "Hmeta_1".
+
+    wp_apply (base.pool_size_spec with "[$]").
+    iSteps.
   Qed.
 
-  Lemma pool_async_silent_spec t ctx task :
+  Lemma pool_async_silent_spec P t ctx scope task :
     {{{
-      pool_context t ctx ∗
-      ( ∀ ctx,
-        pool_context t ctx -∗
+      pool_context t ctx scope ∗
+      ( ∀ ctx scope,
+        pool_context t ctx scope -∗
         WP task ctx {{ res,
-          pool_context t ctx
+          pool_context t ctx scope ∗
+          ▷ □ P
         }}
       )
     }}}
       pool_async_silent ctx task
     {{{
       RET ();
-      pool_context t ctx
+      pool_context t ctx scope ∗
+      pool_obligation t P
     }}}.
   Proof.
     iIntros "%Φ ((:context) & Htask) HΦ".
 
-    wp_rec.
-    wp_pures. rewrite -H𝑐𝑡𝑥_hub.
-
-    awp_apply (ws_hub_std_push_spec with "[$Hhub_inv $Hhub_owner]") without "HΦ"; first done.
-    iInv "Hinv" as "(:inv_inner)".
-    iAaccIntro with "Hhub_model"; first iFrameSteps. iIntros "Hhub_model !>".
-    iSplitL.
-    { iFrame. rewrite big_sepMS_singleton.
-      iIntros "{%} !> %𝑐𝑡𝑥 %empty (:context_consistent) Hhub_owner".
-      wp_apply (wp_wand with "(Htask [Hhub_owner])") as (res) "(:context =1)".
-      { iStep 5. rewrite H𝑐𝑡𝑥_hub. iFrame. }
-      apply (inj context_to_val) in H𝑐𝑡𝑥1_eq as <-.
-      rewrite H𝑐𝑡𝑥_hub. iSteps.
+    wp_apply (base.pool_async_silent_spec P with "[$Hctx Htask]").
+    { iIntros "{%} %ctx %scope Hctx".
+      wp_apply (wp_wand with "(Htask [$Hctx])") as (v) "((:context =1) & $)"; first iSteps.
+      simplify.
+      iDestruct (meta_agree with "Hmeta Hmeta_1") as %->. iClear "Hmeta".
+      iFrame.
     }
-    iIntros "Hhub_owner HΦ".
-
-    iStep 6. rewrite H𝑐𝑡𝑥_hub. iFrame.
+    iSteps.
   Qed.
 
-  Lemma pool_async_spec Ψ Ξ t ctx task :
+  Lemma pool_wait_until_spec P t ctx scope pred :
     {{{
-      pool_context t ctx ∗
-      ( ∀ ctx,
-        pool_context t ctx -∗
-        WP task ctx {{ v,
-          pool_context t ctx ∗
-          ▷ Ψ v ∗
-          ▷ □ Ξ v
-        }}
-      )
-    }}}
-      pool_async ctx task
-    {{{ fut,
-      RET fut;
-      pool_context t ctx ∗
-      pool_future_inv t fut Ψ Ξ ∗
-      pool_future_consumer fut Ψ
-    }}}.
-  Proof.
-    iIntros "%Φ (Hctx & Htask) HΦ".
-
-    wp_rec.
-    wp_smart_apply (ivar_3_create_spec Ψ Ξ with "[//]") as (ivar) "(#Hivar_inv & Hivar_producer & Hivar_consumer)".
-
-    wp_smart_apply (pool_async_silent_spec with "[$Hctx Htask Hivar_producer]") as "Hctx".
-    { clear ctx. iIntros "%ctx Hctx".
-
-      wp_smart_apply (wp_wand with "(Htask Hctx)") as (v) "(Hctx & HΨ & HΞ)".
-      wp_smart_apply (ivar_3_set_spec with "[$Hivar_inv $Hivar_producer $HΨ $HΞ]") as (waiters) "(#Hivar_result & Hwaiters)".
-      wp_smart_apply (lst_iter_spec' (λ _ _, pool_context t ctx)%I with "[$Hctx Hwaiters]") as "$"; try done.
-
-      iApply (big_sepL_impl with "Hwaiters").
-      iIntros "!> %i %waiter %Hwaiters_lookup Hwaiter Hctx".
-      wp_smart_apply (wp_wand with "(Hwaiter [$] [$])") as (res) "(-> & $) //".
-    }
-
-    wp_pures.
-
-    iApply ("HΦ" with "[$]").
-  Qed.
-
-  Lemma pool_wait_until_spec P t ctx pred :
-    {{{
-      pool_context t ctx ∗
+      pool_context t ctx scope ∗
       □ WP pred () {{ res,
         ∃ b,
         ⌜res = #b⌝ ∗
@@ -647,40 +1672,19 @@ Section pool_G.
       pool_wait_until ctx pred
     {{{
       RET ();
-      pool_context t ctx ∗
+      pool_context t ctx scope ∗
       P
     }}}.
   Proof.
-    iIntros "%Φ ((:context lazy=) & #Hpred) HΦ".
-    iLöb as "HLöb".
-    iDestruct "H𝑐𝑡𝑥" as "(:context_1)".
+    iIntros "%Φ ((:context) & Hpred) HΦ".
 
-    wp_rec. rewrite pool_max_round_noyield.
-    wp_smart_apply (wp_wand with "Hpred") as (res) "(%b & -> & HP)".
-    destruct b; first iStepFrameSteps 8.
-
-    awp_smart_apply (ws_hub_std_pop_steal_until_spec P with "[$Hhub_owner $Hpred]") without "HΦ".
-    { lia. }
-    { lia. }
-    { rewrite H𝑐𝑡𝑥_hub //. }
-    iInv "Hinv" as "(:inv_inner)".
-    rewrite -H𝑐𝑡𝑥_hub.
-    iAaccIntro with "Hhub_model"; first iSteps. iIntros ([task |]) "Hhub_model !>"; last first.
-    { iStep 9. iFrame "#∗". rewrite H𝑐𝑡𝑥_hub. iFrameSteps. }
-    iDestruct "Hhub_model" as "(%tasks' & -> & Hhub_model)".
-    iDestruct (big_sepMS_insert with "Htasks") as "(Htask & Htasks')".
-    iSplitR "Htask"; first iSteps.
-    clear empty. iIntros "%empty (Hhub_owner & _) HΦ".
-
-    wp_smart_apply (pool_execute_spec with "[Hhub_owner $Htask]") as (res) "(H𝑐𝑡𝑥 & _)".
-    { iStep 2. rewrite H𝑐𝑡𝑥_hub. iFrame. }
-
-    wp_smart_apply ("HLöb" with "H𝑐𝑡𝑥 HΦ").
+    wp_apply (base.pool_wait_until_spec with "[$]").
+    iSteps.
   Qed.
 
-  Lemma pool_wait_while_spec P t ctx pred :
+  Lemma pool_wait_while_spec P t ctx scope pred :
     {{{
-      pool_context t ctx ∗
+      pool_context t ctx scope ∗
       □ WP pred () {{ res,
         ∃ b,
         ⌜res = #b⌝ ∗
@@ -690,84 +1694,110 @@ Section pool_G.
       pool_wait_while ctx pred
     {{{
       RET ();
-      pool_context t ctx ∗
+      pool_context t ctx scope ∗
       P
     }}}.
   Proof.
-    iIntros "%Φ (Hctx & #Hpred) HΦ".
+    iIntros "%Φ ((:context) & Hpred) HΦ".
 
-    wp_rec.
-    wp_smart_apply (pool_wait_until_spec with "[$Hctx] HΦ"). iModIntro.
-    wp_smart_apply (wp_wand with "Hpred") as (res) "(%b & -> & HP)".
-    destruct b; iSteps.
+    wp_apply (base.pool_wait_while_spec with "[$]").
+    iSteps.
   Qed.
 
-  Lemma pool_wait_spec t ctx fut Ψ Ξ :
+  Lemma pool_async_spec Ψ Ξ t ctx scope task :
     {{{
-      pool_context t ctx ∗
+      pool_context t ctx scope ∗
+      ( ∀ ctx scope,
+        pool_context t ctx scope -∗
+        WP task ctx {{ v,
+          pool_context t ctx scope ∗
+          ▷ Ψ v ∗
+          ▷ □ Ξ v
+        }}
+      )
+    }}}
+      pool_async ctx task
+    {{{ fut,
+      RET fut;
+      pool_context t ctx scope ∗
+      pool_future_inv t fut Ψ Ξ ∗
+      pool_future_consumer fut Ψ ∗
+      pool_obligation t (pool_future_finished fut)
+    }}}.
+  Proof.
+    iIntros "%Φ ((:context) & Htask) HΦ".
+
+    wp_apply (base.pool_async_spec Ψ Ξ with "[$Hctx Htask]").
+    { iIntros "{%} %ctx %scope Hctx".
+      wp_apply (wp_wand with "(Htask [$Hctx])") as (v) "((:context =1) & $)"; first iSteps.
+      simplify.
+      iDestruct (meta_agree with "Hmeta Hmeta_1") as %->. iClear "Hmeta".
+      iFrame.
+    }
+    iSteps.
+  Qed.
+
+  Lemma pool_wait_spec t ctx scope fut Ψ Ξ :
+    {{{
+      pool_context t ctx scope ∗
       pool_future_inv t fut Ψ Ξ
     }}}
       pool_wait ctx fut
     {{{ v,
       RET v;
       £ 2 ∗
-      pool_context t ctx ∗
+      pool_context t ctx scope ∗
       pool_future_result fut v
     }}}.
   Proof.
-    iIntros "%Φ (Hctx & #Hivar_inv) HΦ".
+    iIntros "%Φ ((:context =1) & (:future_inv =2)) HΦ". simplify.
+    iDestruct (meta_agree with "Hmeta_1 Hmeta_2") as %->. iClear "Hmeta_1".
 
-    wp_rec.
-    wp_smart_apply (pool_wait_until_spec (ivar_3_determined fut)%I with "[$Hctx]") as "(Hctx & %v & #Hivar_result)".
-    { iModIntro.
-      wp_smart_apply (ivar_3_is_set_spec with "Hivar_inv") as (b) "Hivar_result".
-      rewrite /ivar_3_determined. destruct b; iSteps.
-    }
-    wp_smart_apply (ivar_3_get_spec with "[$Hivar_inv $Hivar_result]") as "H£".
-    iApply ("HΦ" with "[$]").
+    wp_apply (base.pool_wait_spec with "[$]").
+    iSteps.
   Qed.
 
-  Lemma pool_iter_spec t ctx fut Ψ Ξ fn :
+  Lemma pool_iter_spec t ctx scope fut Ψ Ξ fn :
     {{{
-      pool_context t ctx ∗
+      pool_context t ctx scope ∗
       pool_future_inv t fut Ψ Ξ ∗
-      ( ∀ ctx v,
-        pool_context t ctx -∗
+      ( ∀ ctx scope v,
+        pool_context t ctx scope -∗
         pool_future_result fut v -∗
         WP fn ctx v {{ res,
           ⌜res = ()%V⌝ ∗
-          pool_context t ctx
+          pool_context t ctx scope
         }}
       )
     }}}
       pool_iter ctx fut fn
     {{{
       RET ();
-      pool_context t ctx
+      pool_context t ctx scope
     }}}.
   Proof.
-    iIntros "%Φ (Hctx & #Hivar_inv & Hfn) HΦ".
+    iIntros "%Φ ((:context =1) & (:future_inv =2) & Htask) HΦ". simplify.
+    iDestruct (meta_agree with "Hmeta_1 Hmeta_2") as %->. iClear "Hmeta_1".
 
-    wp_rec.
-    wp_smart_apply (ivar_3_wait_spec with "[$Hivar_inv $Hfn]") as ([v |]) "H".
-    all: wp_pures.
-
-    - iDestruct "H" as "(_ & #Hivar_result & Hfn)".
-      wp_apply (wp_wand with "(Hfn Hctx Hivar_result)") as (res) "(-> & Hctx)".
-      iApply ("HΦ" with "Hctx").
-
-    - iApply ("HΦ" with "Hctx").
+    wp_apply (base.pool_iter_spec with "[$Hctx_1 $Hfut_inv_2 Htask]").
+    { iIntros "{%} %ctx %scope %v Hctx Hfut_inv".
+      wp_apply (wp_wand with "(Htask [$Hctx] [$Hfut_inv])") as (res) "(-> & (:context =3))"; first iSteps.
+      simplify.
+      iDestruct (meta_agree with "Hmeta_2 Hmeta_3") as %->. iClear "Hmeta_2".
+      iFrameSteps.
+    }
+    iSteps.
   Qed.
 
-  Lemma pool_map_spec {t ctx fut1 Ψ1 Ξ1} Ψ2 Ξ2 fn :
+  Lemma pool_map_spec {t ctx scope fut1 Ψ1 Ξ1} Ψ2 Ξ2 fn :
     {{{
-      pool_context t ctx ∗
+      pool_context t ctx scope ∗
       pool_future_inv t fut1 Ψ1 Ξ1 ∗
-      ( ∀ ctx v1,
-        pool_context t ctx -∗
+      ( ∀ ctx scope v1,
+        pool_context t ctx scope -∗
         pool_future_result fut1 v1 -∗
         WP fn ctx v1 {{ v2,
-          pool_context t ctx ∗
+          pool_context t ctx scope ∗
           ▷ Ψ2 v2 ∗
           ▷ □ Ξ2 v2
         }}
@@ -776,38 +1806,31 @@ Section pool_G.
       pool_map ctx fut1 fn
     {{{ fut2,
       RET fut2;
-      pool_context t ctx ∗
+      pool_context t ctx scope ∗
       pool_future_inv t fut2 Ψ2 Ξ2 ∗
       pool_future_consumer fut2 Ψ2
     }}}.
   Proof.
-    iIntros "%Φ (Hctx & #Hfut1_inv & Hfn) HΦ".
+    iIntros "%Φ ((:context =1) & (:future_inv =2) & Htask) HΦ". simplify.
+    iDestruct (meta_agree with "Hmeta_1 Hmeta_2") as %->. iClear "Hmeta_1".
 
-    wp_rec.
-    wp_smart_apply (ivar_3_create_spec Ψ2 Ξ2 with "[//]") as (fut2) "(#Hivar2_inv & Hivar2_producer & Hivar2_consumer)".
-
-    wp_smart_apply (pool_iter_spec with "[$Hctx $Hfut1_inv Hfn Hivar2_producer]") as "Hctx".
-    { clear ctx. iIntros "%ctx %v1 Hctx #Hfut1_result".
-      wp_smart_apply (wp_wand with "(Hfn Hctx Hfut1_result)") as (v2) "(Hctx & HΨ2 & HΞ2)".
-      wp_smart_apply (ivar_3_set_spec with "[$Hivar2_inv $Hivar2_producer $HΨ2 $HΞ2]") as (waiters) "(#Hivar2_result & Hwaiters)".
-      wp_smart_apply (lst_iter_spec' (λ _ _, pool_context t ctx)%I with "[$Hctx Hwaiters]") as "$"; try done.
-      iApply (big_sepL_impl with "Hwaiters").
-      iIntros "!> %i %waiter %Hwaiters_lookup Hwaiter Hctx".
-      wp_smart_apply (wp_wand with "(Hwaiter [$] [$])") as (res) "(-> & $) //".
+    wp_apply (base.pool_map_spec Ψ2 Ξ2 with "[$Hctx_1 $Hfut_inv_2 Htask]").
+    { clear ctx scope. iIntros "%ctx %scope %v1 Hctx Hfut1_inv".
+      wp_apply (wp_wand with "(Htask [$Hctx] [$Hfut1_inv])") as (res) "((:context =3) & $ & $)"; first iSteps.
+      simplify.
+      iDestruct (meta_agree with "Hmeta_2 Hmeta_3") as %->. iClear "Hmeta_2".
+      iFrame.
     }
-
-    wp_pures.
-
-    iApply ("HΦ" with "[$]").
+    iSteps.
   Qed.
 End pool_G.
 
-From zoo_parabs Require
-  pool__opaque.
-
+#[global] Opaque pool_scope.
 #[global] Opaque pool_inv.
 #[global] Opaque pool_model.
 #[global] Opaque pool_context.
+#[global] Opaque pool_obligation.
+#[global] Opaque pool_finished.
 #[global] Opaque pool_future_inv.
 #[global] Opaque pool_future_consumer.
 #[global] Opaque pool_future_result.
