theories/zoo_parabs/pool__code.v
@@ -25,6 +25,10 @@ Definition pool_context : val :=
   fun: "sz" "hub" "id" =>
     ("sz", "hub", "id").
 
+Definition pool_context_main : val :=
+  fun: "t" =>
+    pool_context "t".{size} "t".{hub} #0.
+
 Definition pool_execute : val :=
   fun: "ctx" "job" =>
     "job" "ctx".
@@ -45,6 +49,16 @@ Definition pool_worker : val :=
         "worker" "ctx"
     end.
 
+Definition pool_drain : val :=
+  rec: "drain" "ctx" =>
+    match: ws_hub_std_pop "ctx".<context_hub> "ctx".<context_id> with
+    | None =>
+        ws_hub_std_block "ctx".<context_hub> "ctx".<context_id>
+    | Some "job" =>
+        pool_execute "ctx" "job" ;;
+        "drain" "ctx"
+    end.
+
 Definition pool_create : val :=
   fun: "sz" =>
     let: "hub" := ws_hub_std_create ("sz" + #1) in
@@ -59,16 +73,16 @@ Definition pool_create : val :=
     { "sz", "hub", "domains", () }.
 
 Definition pool_run : val :=
-  fun: "t" "job" =>
+  fun: "t" "task" =>
     ws_hub_std_unblock "t".{hub} #0 ;;
-    let: "res" :=
-      pool_execute (pool_context "t".{size} "t".{hub} #0) "job"
-    in
+    let: "res" := pool_execute (pool_context_main "t") "task" in
     ws_hub_std_block "t".{hub} #0 ;;
     "res".
 
 Definition pool_kill : val :=
   fun: "t" =>
+    ws_hub_std_unblock "t".{hub} #0 ;;
+    pool_drain (pool_context_main "t") ;;
     ws_hub_std_kill "t".{hub} ;;
     array_iter domain_join "t".{domains}.
 
@@ -79,17 +93,6 @@ Definition pool_size : val :=
 Definition pool_async_silent : val :=
   fun: "ctx" "task" =>
     ws_hub_std_push "ctx".<context_hub> "ctx".<context_id> "task".
-
-Definition pool_async : val :=
-  fun: "ctx" "task" =>
-    let: "fut" := ivar_3_create () in
-    pool_async_silent
-      "ctx"
-      (fun: "ctx" =>
-         let: "res" := "task" "ctx" in
-         let: "waiters" := ivar_3_set "fut" "res" in
-         lst_iter (fun: "waiter" => "waiter" "ctx" "res") "waiters") ;;
-    "fut".
 
 Definition pool_wait_until : val :=
   rec: "wait_until" "ctx" "pred" =>
@@ -112,6 +115,17 @@ Definition pool_wait_until : val :=
 Definition pool_wait_while : val :=
   fun: "ctx" "pred" =>
     pool_wait_until "ctx" (fun: <> => ~ "pred" ()).
+
+Definition pool_async : val :=
+  fun: "ctx" "task" =>
+    let: "fut" := ivar_3_create () in
+    pool_async_silent
+      "ctx"
+      (fun: "ctx" =>
+         let: "res" := "task" "ctx" in
+         let: "waiters" := ivar_3_set "fut" "res" in
+         lst_iter (fun: "waiter" => "waiter" "ctx" "res") "waiters") ;;
+    "fut".
 
 Definition pool_wait : val :=
   fun: "ctx" "fut" =>
